Changes:
* Refactoring of field, method, class, ref, var-types for type safety
  and extendability. A few simple bugs were found in preservation (wrong
  eq_dec was used in several places).
* Added multiple frame progress proof cases.

namesAndTypes.v
@@ -32,7 +32,7 @@ Module NamesAndTypesAndOtherNames (ant: AbstractNamesAndTypes) .
   Definition ClassName_type := ant.ClassNameM.t.
   Definition Ref_type := ant.RefM.t.
   Definition v_eq_dec := ant.vn.eq_dec.
-  Definition fn_eq_dec := ant.vn.eq_dec.
+  Definition fn_eq_dec := ant.fn.eq_dec.
   Definition mn_eq_dec := ant.mn.eq_dec.
   Definition cn_eq_dec := ant.cn.eq_dec.
   Definition rn_eq_dec := ant.rn.eq_dec.
@@ -135,22 +135,274 @@ End NamesAndTypesAndOtherNames.
   
 
 Module ConcreteNamesAndTypes <: AbstractNamesAndTypes.
-  Module VarNameM := natT.
-  Module FieldNameM := natT.
-  Module MethodNameM := natT.
-  Module ClassNameM := natT.
-  Module RefM := natT.
 
-  Module natNice <: Nice natT.
-    Definition eq_dec := nat_eq_dec.
-    Definition constructFresh := infiniteNat.constructFresh.
-  End natNice.
+  Module VarNameM.
+    Inductive _var_name_type :=
+    | _var_name_type_constr : nat -> _var_name_type.
+    Definition t := _var_name_type.
+  End VarNameM.
 
-  Module vn := natNice.
-  Module fn := natNice.
-  Module mn := natNice.
-  Module cn := natNice.
-  Module rn := natNice.
+  Module FieldNameM.
+    Inductive _field_name_type :=
+    | _field_name_type_constr : nat -> _field_name_type.
+    Definition t := _field_name_type.
+  End FieldNameM.
+
+  Module MethodNameM.
+    Inductive _method_name_type :=
+    | _method_name_type_constr : nat -> _method_name_type.
+    Definition t := _method_name_type.
+  End MethodNameM.
+
+  Module ClassNameM.
+    Inductive _class_name_type :=
+    | _class_name_type_constr : nat -> _class_name_type.
+    Definition t := _class_name_type.
+  End ClassNameM.
+
+  Module RefM.
+    Inductive _ref_type :=
+    | _ref_type_constr : nat -> _ref_type.
+    Definition t := _ref_type.
+  End RefM.
+
+  
+
+  Module varNameNice <: Nice VarNameM.
+    Import VarNameM.
+    Lemma _var_name_eq_dec :
+      forall (x y : _var_name_type),
+        {x = y} + {x <> y}.
+      intros.
+      destruct x as [nx]; destruct y as [ny].
+      case_eq (nat_eq_dec nx ny); intros; clear H.
+      left; rewrite e; reflexivity.
+      right; simplify_eq; assumption.
+    Qed.
+    Definition eq_dec := _var_name_eq_dec.
+    
+
+    Require Import Coq.Lists.List.
+
+    Lemma _var_name_type_constructFresh
+     : forall lT : list _var_name_type,
+         {fresh : _var_name_type | ~ In fresh lT}.
+      Definition unpack (x: _var_name_type) :=
+        match x with | _var_name_type_constr nx => nx end.
+      intros.
+      set (lTn := map unpack lT).
+      destruct (infiniteNat.constructFresh lTn) as [fresh_nat fresh_nat_is_fresh].
+
+      
+      assert (forall x1 x2, unpack x1 = unpack x2 -> x1 = x2) as unpack_injective.
+      intros.
+      destruct x1 as [n1]; destruct x2 as [n2].
+      simplify_eq H; intro are_eq; rewrite are_eq; reflexivity.
+      
+      set (lem := count_occ_map unpack _var_name_eq_dec nat_eq_dec unpack_injective
+                                (_var_name_type_constr fresh_nat) lT
+          ).
+      fold lTn in lem.
+      simpl in lem.
+      set (lemlem := proj1 (count_occ_not_In nat_eq_dec lTn fresh_nat) fresh_nat_is_fresh).
+      rewrite lemlem in lem.
+      set (lemlemlem := proj2 (count_occ_not_In _var_name_eq_dec lT (_var_name_type_constr fresh_nat))
+                              lem).
+      exact (exist _ (_var_name_type_constr fresh_nat) lemlemlem).
+    Qed.
+      
+    Definition constructFresh := _var_name_type_constructFresh.
+  End varNameNice.
+
+  Module fieldNameNice <: Nice FieldNameM.
+    Import FieldNameM.
+    Lemma _field_name_eq_dec :
+      forall (x y : _field_name_type),
+        {x = y} + {x <> y}.
+      intros.
+      destruct x as [nx]; destruct y as [ny].
+      case_eq (nat_eq_dec nx ny); intros; clear H.
+      left; rewrite e; reflexivity.
+      right; simplify_eq; assumption.
+    Qed.
+    Definition eq_dec := _field_name_eq_dec.
+    
+
+    Require Import Coq.Lists.List.
+
+    Lemma _field_name_type_constructFresh
+     : forall lT : list _field_name_type,
+         {fresh : _field_name_type | ~ In fresh lT}.
+      Definition unpack (x: _field_name_type) :=
+        match x with | _field_name_type_constr nx => nx end.
+      intros.
+      set (lTn := map unpack lT).
+      destruct (infiniteNat.constructFresh lTn) as [fresh_nat fresh_nat_is_fresh].
+
+      
+      assert (forall x1 x2, unpack x1 = unpack x2 -> x1 = x2) as unpack_injective.
+      intros.
+      destruct x1 as [n1]; destruct x2 as [n2].
+      simplify_eq H; intro are_eq; rewrite are_eq; reflexivity.
+      
+      set (lem := count_occ_map unpack _field_name_eq_dec nat_eq_dec unpack_injective
+                                (_field_name_type_constr fresh_nat) lT
+          ).
+      fold lTn in lem.
+      simpl in lem.
+      set (lemlem := proj1 (count_occ_not_In nat_eq_dec lTn fresh_nat) fresh_nat_is_fresh).
+      rewrite lemlem in lem.
+      set (lemlemlem := proj2 (count_occ_not_In _field_name_eq_dec lT (_field_name_type_constr fresh_nat))
+                              lem).
+      exact (exist _ (_field_name_type_constr fresh_nat) lemlemlem).
+    Qed.
+      
+    Definition constructFresh := _field_name_type_constructFresh.
+  End fieldNameNice.
+
+  Module methodNameNice <: Nice MethodNameM.
+    Import MethodNameM.
+    Lemma _method_name_eq_dec :
+      forall (x y : _method_name_type),
+        {x = y} + {x <> y}.
+      intros.
+      destruct x as [nx]; destruct y as [ny].
+      case_eq (nat_eq_dec nx ny); intros; clear H.
+      left; rewrite e; reflexivity.
+      right; simplify_eq; assumption.
+    Qed.
+    Definition eq_dec := _method_name_eq_dec.
+    
+
+    Require Import Coq.Lists.List.
+
+    Lemma _method_name_type_constructFresh
+     : forall lT : list _method_name_type,
+         {fresh : _method_name_type | ~ In fresh lT}.
+      Definition unpack (x: _method_name_type) :=
+        match x with | _method_name_type_constr nx => nx end.
+      intros.
+      set (lTn := map unpack lT).
+      destruct (infiniteNat.constructFresh lTn) as [fresh_nat fresh_nat_is_fresh].
+
+      
+      assert (forall x1 x2, unpack x1 = unpack x2 -> x1 = x2) as unpack_injective.
+      intros.
+      destruct x1 as [n1]; destruct x2 as [n2].
+      simplify_eq H; intro are_eq; rewrite are_eq; reflexivity.
+      
+      set (lem := count_occ_map unpack _method_name_eq_dec nat_eq_dec unpack_injective
+                                (_method_name_type_constr fresh_nat) lT
+          ).
+      fold lTn in lem.
+      simpl in lem.
+      set (lemlem := proj1 (count_occ_not_In nat_eq_dec lTn fresh_nat) fresh_nat_is_fresh).
+      rewrite lemlem in lem.
+      set (lemlemlem := proj2 (count_occ_not_In _method_name_eq_dec lT (_method_name_type_constr fresh_nat))
+                              lem).
+      exact (exist _ (_method_name_type_constr fresh_nat) lemlemlem).
+    Qed.
+      
+    Definition constructFresh := _method_name_type_constructFresh.
+  End methodNameNice.
+
+  Module classNameNice <: Nice ClassNameM.
+    Import ClassNameM.
+    Lemma _class_name_eq_dec :
+      forall (x y : _class_name_type),
+        {x = y} + {x <> y}.
+      intros.
+      destruct x as [nx]; destruct y as [ny].
+      case_eq (nat_eq_dec nx ny); intros; clear H.
+      left; rewrite e; reflexivity.
+      right; simplify_eq; assumption.
+    Qed.
+    Definition eq_dec := _class_name_eq_dec.
+    
+
+    Require Import Coq.Lists.List.
+
+    Lemma _class_name_type_constructFresh
+     : forall lT : list _class_name_type,
+         {fresh : _class_name_type | ~ In fresh lT}.
+      Definition unpack (x: _class_name_type) :=
+        match x with | _class_name_type_constr nx => nx end.
+      intros.
+      set (lTn := map unpack lT).
+      destruct (infiniteNat.constructFresh lTn) as [fresh_nat fresh_nat_is_fresh].
+
+      
+      assert (forall x1 x2, unpack x1 = unpack x2 -> x1 = x2) as unpack_injective.
+      intros.
+      destruct x1 as [n1]; destruct x2 as [n2].
+      simplify_eq H; intro are_eq; rewrite are_eq; reflexivity.
+      
+      set (lem := count_occ_map unpack _class_name_eq_dec nat_eq_dec unpack_injective
+                                (_class_name_type_constr fresh_nat) lT
+          ).
+      fold lTn in lem.
+      simpl in lem.
+      set (lemlem := proj1 (count_occ_not_In nat_eq_dec lTn fresh_nat) fresh_nat_is_fresh).
+      rewrite lemlem in lem.
+      set (lemlemlem := proj2 (count_occ_not_In _class_name_eq_dec lT (_class_name_type_constr fresh_nat))
+                              lem).
+      exact (exist _ (_class_name_type_constr fresh_nat) lemlemlem).
+    Qed.
+      
+    Definition constructFresh := _class_name_type_constructFresh.
+  End classNameNice.
+
+  Module refNice <: Nice RefM.
+    Import RefM.
+    Lemma _ref_eq_dec :
+      forall (x y : _ref_type),
+        {x = y} + {x <> y}.
+      intros.
+      destruct x as [nx]; destruct y as [ny].
+      case_eq (nat_eq_dec nx ny); intros; clear H.
+      left; rewrite e; reflexivity.
+      right; simplify_eq; assumption.
+    Qed.
+    Definition eq_dec := _ref_eq_dec.
+    
+    Require Import Coq.Lists.List.
+
+    Lemma _ref_type_constructFresh
+     : forall lT : list _ref_type,
+         {fresh : _ref_type | ~ In fresh lT}.
+      Definition unpack (x: _ref_type) :=
+        match x with | _ref_type_constr nx => nx end.
+      intros.
+      set (lTn := map unpack lT).
+      destruct (infiniteNat.constructFresh lTn) as [fresh_nat fresh_nat_is_fresh].
+
+      
+      assert (forall x1 x2, unpack x1 = unpack x2 -> x1 = x2) as unpack_injective.
+      intros.
+      destruct x1 as [n1]; destruct x2 as [n2].
+      simplify_eq H; intro are_eq; rewrite are_eq; reflexivity.
+      
+      set (lem := count_occ_map unpack _ref_eq_dec nat_eq_dec unpack_injective
+                                (_ref_type_constr fresh_nat) lT
+          ).
+      fold lTn in lem.
+      simpl in lem.
+      set (lemlem := proj1 (count_occ_not_In nat_eq_dec lTn fresh_nat) fresh_nat_is_fresh).
+      rewrite lemlem in lem.
+      set (lemlemlem := proj2 (count_occ_not_In _ref_eq_dec lT (_ref_type_constr fresh_nat))
+                              lem).
+      exact (exist _ (_ref_type_constr fresh_nat) lemlemlem).
+    Qed.
+      
+    Definition constructFresh := _ref_type_constructFresh.
+  End refNice.
+
+  Module vn := varNameNice.
+  Module fn := fieldNameNice.
+  Module mn := methodNameNice.
+  Module rn := refNice.
+  Module cn := classNameNice.
+  
 End ConcreteNamesAndTypes.
 
 Module ConcreteEverything := NamesAndTypesAndOtherNames ConcreteNamesAndTypes.
