progress_sf.v
@@ -1,0 +1,361 @@
+(*
+progress: 
+ *)
+Require Import syntax.
+Require Import partial.
+Require Import heap.
+Require Import classTable.
+Require Import sframe.
+Require Import reductions.
+Require Import typing.
+Require Import namesAndTypes.
+
+Require Import wf_env.
+
+Import ConcreteEverything.
+
+
+Section Progress_SF.
+
+  Variable P: Program.
+
+  Definition subtypeP := subtype P.
+  Definition fldP := fld P.
+  Definition ftypeP := ftype P.
+  Definition t_frame1' := t_frame1 P.
+  Definition WF_Frame' := WF_Frame P.
+
+  Definition Reduction_SF' := Reduction_SF P .
+  Definition fieldsP := fields P.
+  Definition TypeChecksP := TypeChecks P.
+  Definition Heap_okP := Heap_ok P.
+  Definition Heap_dom_okP := Heap_dom_ok P .
+
+  Notation "( p +++ a --> b )" := (p_env.updatePartFunc
+                                     p a b) (at level 0).
+
+  Notation "( H +*+ o --> obj )" := (p_heap.updatePartFunc
+                                              H o obj)
+                                      (at level 0).
+
+  Theorem progress_SF_case_new :
+    forall H L C t x sigma ann,
+      WF_Frame' H (ann_frame
+                     (sframe L (t_let x <- New C t_in (t)))
+                     ann) sigma ->
+      Heap_okP H ->
+      Heap_dom_okP H ->
+      { frame : sfconfig_type
+                  & Reduction_SF'
+                  (# H, L, t_let x <- New C t_in (t) !)
+                  frame}.
+    Proof.
+      intros.
+      inversion X.
+      clear H2 H4 L0 H3 t0 H6 ann0 H7 sigma0 H5.
+
+      (* define flds *)
+      set (flds := fieldsList P C).
+      set (C_flds := fieldsListIsFields P C).
+      fold flds in C_flds.
+      set (FM := p_FM.newPartFunc flds FM_null).
+            
+      destruct (ConcreteNamesAndTypes.rn.constructFresh
+                  (p_heap.domain H))
+        as [o o_fresh_prop].
+      
+      exists ( # (H +*+ o --> (obj C FM)),
+               ( L +++ x --> envRef o ) , t ! ).
+      apply (E_New _ _ _ _ _ _  _ _  flds).
+      inversion H8.
+      assumption; clear H2 H3.
+      assumption.
+      assumption.
+      reflexivity.
+    Qed.
+
+    Theorem progress_SF_case_box :
+    forall H L C t x sigma ann,
+      WF_Frame' H (ann_frame
+                     (sframe L (t_let x <- Box C t_in (t)))
+                     ann) sigma ->
+      Heap_okP H ->
+      Heap_dom_okP H ->
+      { frame : sfconfig_type
+                  & Reduction_SF'
+                  (# H, L, t_let x <- Box C t_in (t) !)
+                  frame}.
+    Proof.
+      intros.
+      inversion X.
+      clear H2 H4 L0 H3 t0 H6 ann0 H7 sigma0 H5.
+
+      (* define flds *)
+      set (flds := fieldsList P C).
+      set (C_flds := fieldsListIsFields P C).
+      fold flds in C_flds.
+      set (FM := p_FM.newPartFunc flds FM_null).
+            
+      destruct (ConcreteNamesAndTypes.rn.constructFresh
+                  (p_heap.domain H))
+        as [o o_fresh_prop].
+      
+      exists ( # (H +*+ o --> (obj C FM)),
+               ( L +++ x --> envBox o ) , t ! ).
+      apply (E_Box _ _ _ _ _ _  _ _  flds).
+      inversion H8.
+      assumption; clear H2 H3.
+      assumption.
+      assumption.
+      reflexivity.
+    Qed.
+
+
+    Theorem progress_SF_case_var :
+    forall H L t x y sigma ann,
+      WF_Frame' H (ann_frame
+                     (sframe L (t_let x <- (Var y) t_in t))
+                     ann) sigma ->
+      Heap_okP H ->
+      Heap_dom_okP H ->
+      { frame : sfconfig_type
+                  & Reduction_SF'
+                  (# H, L, (t_let x <- (Var y) t_in t) !)
+                  frame}.
+    Proof.
+      intros.
+      inversion X.
+      clear H2 H4 L0 H3 t0 H6 ann0 H7 sigma0 H5.
+      
+      assert ({null_ref_box | p_env.func L y = Some null_ref_box}).
+      clear H8 H1 H0 X ann.
+      inversion X0.
+      clear H0 gamma H1 eff0 x0 H3 t0 H5 tau H2 e H4.
+      inversion X.
+      clear H1 eff0 x0 H4 sigma1 H2 H0 X X2 gamma X0.
+      apply fst in X1.
+      unfold gamma_env_subset in X1.
+      apply (fun f => f y) in X1.
+      apply (fun f => f (p_gamma.in_part_func_domain _ _ _ H3)) in X1.
+      case_eq (p_env.func L y).
+      intros L_y L_y_eq.
+      exists L_y; reflexivity.
+      intro.
+      set (lem := p_env.fDomainCompat L y).
+      firstorder.
+      
+      destruct X2 as [null_ref_box L_y_is_null_ref_box].
+      
+      exists ( # H , (L +++ x --> null_ref_box) , t ! ).
+      apply E_Var.
+      inversion H8.
+      assumption.
+      assumption.
+    Qed.
+
+    Theorem progress_SF_case_null :
+    forall H L t x sigma ann,
+      WF_Frame' H (ann_frame
+                     (sframe L (t_let x <- Null t_in t))
+                     ann) sigma ->
+      Heap_okP H ->
+      Heap_dom_okP H ->
+      { frame : sfconfig_type
+                  & Reduction_SF'
+                  (# H, L, (t_let x <- Null t_in t) !)
+                  frame}.
+    Proof.
+      intros.
+
+      exists (# H, (L +++ x --> envNull), t !).
+      apply E_Null.
+      
+      inversion X.
+      clear H2 H4 L0 H3 t0 H6 ann0 H7 sigma0 H5 X0 X1 eff Gamma H1 H0 X ann
+      sigma P H L .
+      inversion H8.
+      assumption.
+    Qed.
+
+    Theorem progress_SF_case_field :
+    forall H L t x y f sigma ann,
+      WF_Frame' H (ann_frame
+                     (sframe L (t_let x <- (FieldSelection y f) t_in t))
+                     ann) sigma ->
+      p_env.func L y <> Some envNull ->
+      Heap_okP H ->
+      Heap_dom_okP H ->
+      { frame : sfconfig_type
+                  & Reduction_SF'
+                  (# H, L, (t_let x <- (FieldSelection y f) t_in t) !)
+                  frame}.
+      intros.
+      rename H0 into L_y_not_null.
+      rename H2 into heap_dom_ok.
+      inversion X.
+      inversion H7.
+      rename H9 into t_is_term.
+      clear H8 H7.
+      clear H0 H2  H4 L0 H3 t0 H6 ann0 sigma0 H5 H4.
+      assert ({C | p_gamma.func Gamma y = Some (typt_class C)}).
+      clear H1  X ann.
+      inversion X0.
+      clear  H0 gamma H1 eff0 x0 H3 t0 H5 tau H2 e H4 x X0 X2 sigma .
+      inversion X.
+      clear H0 eff0 x f0 H1 H2  H4 gamma H3 sigma0 X witn t t_is_term f.
+      exists C; assumption.
+      destruct X2 as [C gamma_y_is_C].
+
+      Require Import Coq.Lists.List.
+
+      assert ({o | p_env.func L y = Some (envRef o) /\
+                   In o (p_heap.domain H)
+              }).
+
+      destruct X1 as [subset L_gamma_compat].
+      unfold gamma_env_subset in subset.
+      apply (fun f => f y) in subset.
+      apply (fun f => f (p_gamma.in_part_func_domain _ _ _ gamma_y_is_C)) in subset.
+      apply (fun f => f y (typt_class C) gamma_y_is_C) in L_gamma_compat.
+      
+      case_eq (p_env.func L y).
+      intros L_y L_y_eq.
+      destruct L_y.
+      firstorder.
+      exists r. split. reflexivity.
+
+      destruct L_gamma_compat.
+      destruct s.
+      firstorder.
+      destruct s as [aa bb]; destruct aa as [cc oo]; destruct bb as [aaa bbb];
+      destruct bbb as [aaaa bbbb].
+      rewrite L_y_eq in aaaa.
+      inversion aaaa.
+      rewrite H2 in *.
+      assumption.
+      
+      destruct s as [aa bb]; destruct aa as [cc oo]; destruct bb as [aaa bbb];
+      destruct bbb as [aaaa bbbb]; destruct bbbb as [aaaaa bbbbb].
+      rewrite gamma_y_is_C in aaaaa.
+      discriminate.
+
+      destruct L_gamma_compat.
+      destruct s.
+      firstorder.
+      destruct s as [aa bb]; destruct aa as [cc oo]; destruct bb as [aaa bbb];
+      destruct bbb as [aaaa bbbb].
+      rewrite L_y_eq in aaaa; discriminate.
+
+      destruct s as [aa bb]; destruct aa as [cc oo]; destruct bb as [aaa bbb];
+      destruct bbb as [aaaa bbbb]; destruct bbbb as [aaaaa bbbbb].
+      rewrite gamma_y_is_C in aaaaa.
+      discriminate.
+
+      intro.
+      set (lem := p_env.fDomainCompat L y).
+      firstorder.
+
+      destruct X2 as [o L_y_i_o].
+
+      inversion X0.
+      clear tau H3 t0 H6 e H5 x0 H4 eff0 H2 gamma H0 X3.
+      inversion X2.
+      clear  H5 f0 H0 x0 H3 eff0 H2 gamma.
+      clear H4 X2 sigma0.
+      rewrite  gamma_y_is_C in H6.
+      inversion H6.
+      rewrite <- H2 in *.
+      clear C0 H2 H6.
+      rename C into C'.
+
+      destruct X1 as [_ L_gamma_compat].
+      apply (fun f => f y (typt_class C') gamma_y_is_C) in L_gamma_compat.
+      destruct L_y_i_o as [L_y_i_o o_in_H].
+      assert ({C | heap_typeof H o o_in_H = C /\
+                   subclass P C C'
+              }).
+      
+      destruct L_gamma_compat.
+      destruct s.
+      firstorder.
+      destruct s as [aa bb]; destruct aa as [cc oo]; destruct bb as [aaa bbb];
+      destruct bbb as [aaaa bbbb]; destruct bbbb as [aaaaa bbbbb].
+      rewrite gamma_y_is_C in aaaaa.
+      inversion aaaaa.
+      rewrite <- H2 in *.
+      clear H2 aaaaa cc.
+      rewrite L_y_i_o in aaaa; inversion aaaa.
+      rewrite  H2 in *.
+      clear aaaa.
+      exists (heap_typeof H oo aaa).
+      split.
+
+      set (C := heap_typeof H o o_in_H).
+      destruct (heap_typeof_impl P H o C o_in_H (eq_refl _))
+        as [FM H_o_value].
+      rewrite H2 in H_o_value.
+      symmetry.
+      apply (heap_typeof_same P _ _ _ FM H_o_value).
+      unfold wf_env.subtypeP in bbbbb.
+      inversion bbbbb.
+      clear D H0 H3      .
+      assumption.
+      
+      destruct s as [aa bb]; destruct aa as [cc oo]; destruct bb as [aaa bbb];
+      destruct bbb as [aaaa bbbb]; destruct bbbb as [aaaaa bbbbb].
+      rewrite gamma_y_is_C in aaaaa.
+      discriminate.
+
+      unfold Heap_dom_okP in heap_dom_ok.
+      destruct X1 as [C heap_tpe_tmp].
+      destruct heap_tpe_tmp as [typeof_o_C C_sub_C'].
+      
+      destruct (heap_typeof_impl P _ _ _ o_in_H typeof_o_C) as [FM H_o_value].
+      
+      apply (fun f => f o C FM ) in heap_dom_ok.
+      apply (fun f => f H_o_value) in heap_dom_ok.
+      unfold heap.fieldsP in heap_dom_ok.
+
+      (* goal: *)
+      assert (typing.fldP P C f).
+      apply (field_subclass P C C'); assumption.
+      
+      clear L_gamma_compat X0 C' gamma_y_is_C  witn C_sub_C' X L_y_not_null
+            H1   Gamma eff   .
+
+      set (lem := fld_in_flds P C f (p_FM.domain FM) H0 heap_dom_ok).
+
+      assert ({fmVal | p_FM.func FM f = Some fmVal}).
+      case_eq (p_FM.func FM f).
+      intro fmVal; exists fmVal; reflexivity.
+      intro.
+      set (lemlem := p_FM.fDomainCompat FM f).
+      firstorder.
+
+      destruct X as [fmVal FM_f].
+      exists      
+      ( # H,
+        ( L +++ x --> (fm2env fmVal) ) , t ! ).
+
+      apply (E_Field _ _ _ o _ _ _ _
+                     C FM _ t_is_term L_y_i_o H_o_value
+                     FM_f
+            ).
+    Qed.
+
+
+    Theorem progress_SF_case_assign :
+    forall H L t x y f z sigma ann,
+      WF_Frame' H (ann_frame
+                     (sframe L (t_let x <- (FieldAssignment y f z) t_in t))
+                     ann) sigma ->
+      p_env.func L y <> Some envNull ->
+      Heap_okP H ->
+      Heap_dom_okP H ->
+      { frame : sfconfig_type
+                  & Reduction_SF'
+                  (# H, L, (t_let x <- (FieldAssignment y f z) t_in t) !)
+                  frame}.
+    Admitted.
+
+End Progress_SF.
